More PEquiv

src/experiments/PEquiv.v
@@ -1,13 +1,3 @@
-(* Notes
-- loading each state of a SOS execution produces an execution that technically
-  isn't a abstract machine execution -- suggests we might not want to limit
-  ourselves to the type of machine executions
-- alternatively, it might be necessary to define the machine induced by the
-  the SOS step relation on machine states. That is, where the step function is
-  load o SOS.step o unload
-*)
-
-
 Generalizable All Variables.
 Set Implicit Arguments.
 
@@ -20,109 +10,6 @@ Record Equiv {A} (R:A -> A -> Prop) :=
   ; equiv_sym : forall a b, R a b -> R b a
   ; equiv_trans : forall a b c, R a b -> R b c -> R a c
   }.
-
-CoInductive stream X := 
-  Stream { s_hd : X
-         ; s_tl : option (stream X)
-         }.
-
-Definition stream_id {X} (s:stream X) : stream X :=
-  let 'Stream hd tl := s in
-  Stream hd tl.
-
-Lemma stream_id_eq X : forall s : stream X,
-  s = stream_id s.
-Proof.
-  intro. destruct s. simpl. reflexivity.
-Qed.
-
-CoFixpoint map_stream {X Y} (f:X -> Y) (s:stream X) : stream Y :=
-  match s with
-  | Stream hd None => Stream (f hd) None
-  | Stream hd (Some tl) => Stream (f hd) (Some (map_stream f tl))
-  end.
-
-Inductive fbisim_step {X Y} (R:stream X -> stream X -> Prop) (U:X -> Y) 
-  : stream X -> stream X -> Prop :=
-| ueq_one : forall x x',
-    U x = U x' ->
-    fbisim_step R U {| s_hd := x; s_tl := None |} 
-                    {| s_hd := x'; s_tl := None |}
-| ueq_step : forall x x' s' t',
-    U x = U x' ->
-    R s' t' ->
-    fbisim_step R U {| s_hd := x; s_tl := Some s' |} 
-                    {| s_hd := x'; s_tl := Some t' |}.
-
-
-CoInductive fbisim {X Y} (U:X->Y) (s t:stream X) : Prop :=
-fbism_fix : 
-  fbisim_step (fbisim U) U s t ->
-  fbisim U s t.
-
-Section FBISIM_COIND.
-
-  Variables (X Y:Type) (U:X -> Y) (R:stream X -> stream X -> Prop).
-
-  Hypothesis H : forall s t, R s t -> fbisim_step R U s t.
-  
-  Lemma fbisim_coind : forall s t,
-    R s t -> fbisim U s t.
-  Proof.
-    cofix CIH.
-    intros s t Hrst. 
-    destruct s as [? [s'|]], t as [? [t'|]]; apply H in Hrst; inversion Hrst; subst.
-    - constructor. constructor. assumption. apply CIH. assumption.
-    - constructor. constructor. assumption.
-  Qed.
-
-End FBISIM_COIND.
-
-Section STREAM_REL_QUOT.
-
-Variables (X Y:Type) (U:X -> Y) (L:Y -> X).
-Hypothesis Hepi : forall y, U (L y) = y.
-
-Lemma unload_load_R : forall s,
-  fbisim U (map_stream L (map_stream U s)) s.
-Proof.
-  intros s.
-  eapply fbisim_coind with (R:=fun s t => s = (map_stream L (map_stream U t))).
-  - intros s' t ?; subst s'.
-    destruct t as [? [t'|]]. 
-    + rewrite stream_id_eq at 1. simpl. constructor.
-      rewrite Hepi. reflexivity. reflexivity.
-    + rewrite stream_id_eq at 1. simpl. constructor.
-      rewrite Hepi. reflexivity. 
-  - reflexivity.
-Qed.
-
-Variable R : stream X -> stream X -> Prop.
-Hypothesis Hequiv : Equiv R.
-Hypothesis Hincl : forall s t, fbisim U s t -> R s t.
-
-Theorem stream_rel_quot :
-  forall s t, R s t <-> R (map_stream L (map_stream U s))
-                          (map_stream L (map_stream U t)).
-Proof.
-  intros s t. split.
-  + intros HRst. 
-    eapply (equiv_trans Hequiv). apply Hincl. apply unload_load_R.
-    eapply (equiv_trans Hequiv). apply HRst.
-    eapply (equiv_sym Hequiv). apply Hincl. apply unload_load_R.
-  + intros HRst.
-    eapply (equiv_trans Hequiv). apply (equiv_sym Hequiv). apply Hincl. apply unload_load_R.
-    eapply (equiv_trans Hequiv). apply HRst.
-    apply Hincl. apply unload_load_R.
-Qed.
-  
-End STREAM_REL_QUOT.
-
-(* The above formulation of program equivalence isn't flexible enough to
-   define, for example, terminal states that act as input, or variations
-   of applicative similarity. It only inspects the sequence of states
-   starting from the intial state: the observer can't "call back into the
-   interpreter" to further examine terminal states. *)
 
 Record State :=
   { st_ty :> Type
@@ -139,6 +26,7 @@ Record Mach (X:State) :=
       end
   }.
 
+(* Homomorphic embedding *)
 Record HEmbed `(M:Mach X, N:Mach Y) :=
   { he_U : X -> Y
   ; he_U_wf : forall x, st_wf X x -> st_wf Y (he_U x)
@@ -149,25 +37,26 @@ Record HEmbed `(M:Mach X, N:Mach Y) :=
     option_map he_U (m_step M x) = m_step N (he_U x)
   }.
 
+(* Simulation between machines (partial fns on states) *)
+Definition mach_sim {X:State} (R:X -> X -> Prop) (M M':Mach X) : Prop :=
+  forall x x', st_wf X x -> st_wf X x' -> 
+    R x x' -> 
+    match m_step M x, m_step M' x' with
+    | Some y, Some y' => R y y'
+    | None, None => True
+    | _, _ => False
+    end.
 
-Definition PEq_respects X Y 
-           (PEq : Mach X -> X -> X -> Prop)
-           (U:X -> Y) : Prop :=
-  forall (M M':Mach X)
-    (Hsim : forall x x' (Hwfx:st_wf X x) (Hwfx':st_wf X x'),
-        U x = U x' -> 
-        option_map U (m_step M x) = option_map U (m_step M' x')),
-  forall x x' (Hwfx:st_wf X x) (Hwfx':st_wf X x'),
-    PEq M x x' <-> PEq M' x x'.
-
-
-Section GEN_PROG_EQ.
+(* The main point is that when the "machine equivalence" diagram H
+   between a machine M and a "more abstract" machine N, we have an
+   induced machine "hembed_mach H" defined in terms of the transitions
+   N, loading and unloading, where the equivalence induced by
+   unloading is a simulation between M and hembed_mach H. *)
+Section HEMBED_SIM.
 
 Context `(M:Mach X, N:Mach Y, H:HEmbed M N).
 
-Variable PEq : Mach X -> X -> X -> Prop.
-
-Let M' : Mach X.
+Definition hembed_mach : Mach X.
   refine
     {| m_step x := option_map (he_L H) (m_step N (he_U H x)) |}.
 Proof.
@@ -177,25 +66,181 @@ Proof.
      [ simpl; apply (he_L_wf H) | ]; auto).
 Defined.
 
-Theorem gen_prog_eq : forall x x' (Hwfx:st_wf X x) (Hwfx':st_wf X x')
-    (HPeq_usim:PEq_respects PEq (he_U H)),
-    PEq M x x' <-> PEq M' x x'.
+Lemma hembed_sim :
+  mach_sim (fun x x' => he_U H x = he_U H x') M hembed_mach.
 Proof.
-  split.
-  - eapply HPeq_usim; auto. clear x x' Hwfx Hwfx'.
-    intros. subst M'. simpl. 
-    rewrite (he_spec H); auto. rewrite H0.
-    apply (he_U_wf H) in Hwfx'.
-    apply (m_pres N) in Hwfx'.
-    destruct (m_step N (he_U H x')) as [y'|] eqn:Heqy; auto.
-    simpl. rewrite (he_epi H); auto.
-  - eapply HPeq_usim; auto. clear x x' Hwfx Hwfx'.
-    intros. subst M'. simpl.
-    rewrite (he_spec H); auto. rewrite H0.
-    apply (he_U_wf H) in Hwfx'.
-    apply (m_pres N) in Hwfx'.
-    destruct (m_step N (he_U H x')) as [y'|] eqn:Heqy; auto.
-    simpl. rewrite (he_epi H); auto.
+  unfold hembed_mach, mach_sim. simpl.
+  intros ? ? Hx Hx' Hxx'.
+  destruct (m_step M x) eqn:Hstep, (m_step N (he_U H x')) eqn:Hstep';
+    simpl; auto.
+  - rewrite <- Hxx' in Hstep'.
+    rewrite <- (he_spec H) in Hstep'; auto.
+    rewrite Hstep in Hstep'. inversion Hstep'; subst s0.
+    rewrite (he_epi H); auto. 
+    eapply (he_U_wf H). 
+    apply (m_pres M) in Hx. rewrite Hstep in Hx. assumption.
+  - rewrite <- Hxx' in Hstep'.
+    rewrite <- (he_spec H) in Hstep'; auto.
+    rewrite Hstep in Hstep'. simpl in *. congruence.
+  - rewrite <- Hxx' in Hstep'.
+    rewrite <- (he_spec H) in Hstep'; auto.
+    rewrite Hstep in Hstep'. simpl in *. congruence.
 Qed.
 
-End GEN_PROG_EQ.
+End HEMBED_SIM.
+
+
+(* To use the above fact, for example to replace reasoning about
+   equivalence of abstract machine programs with SOS, we would first
+   have to show that the property we want to reason about doesn't
+   depend on the "intensional details" of states that are quotiented
+   out by unloading. I.E. we're only observing the transition system
+   up to machine simulation. Then, whatever we want to show about
+   the abstract machine (e.g. an instance of some program equivalence)
+   can instead be proven using SOS transitions.
+
+   Note that unloading and loading do essentially nothing for initial
+   states. For example, in a CEK-like machine 
+   (c, [], []) -> c -> (c, [], [])
+   So the traces of the "induced" machine are just the SOS. We don't
+   have to worry about proving things about unloading. *)
+Section P_QUOT_HEMBED.
+
+Context `(P:Mach X -> Prop, M:Mach X, N:Mach Y, H:HEmbed M N).
+
+Hypothesis Pinv : forall (M M':Mach X),
+  mach_sim (fun x x' => he_U H x = he_U H x') M M' ->
+  (P M <-> P M').
+
+Lemma p_quot_hembed : P M <-> P (hembed_mach H).
+Proof.
+  apply Pinv. apply hembed_sim.
+Qed.
+
+End P_QUOT_HEMBED.
+
+
+(* TODO: Actual CEK machine is a bit too tricky ... 
+   easier example from mini branch? *)
+Section EXAMPLES.
+
+Inductive tm :=
+| Var : nat -> tm
+| Lam : tm -> tm
+| App : tm -> tm -> tm.
+
+Scheme Equality for tm.
+
+Fixpoint csubst (x:nat) (m v:tm) : tm :=
+  match m with
+  | Var y => if eq_nat_dec x y then v else (Var y)
+  | Lam m => Lam (csubst (S x) m v)
+  | App m n => App (csubst x m v) (csubst x n v)
+  end.
+
+Fixpoint sos_step (m:tm) : option tm :=
+  match m with
+  | Var x => None
+  | Lam x => None
+  | App (Lam m) (Lam n) => Some (csubst 0 m (Lam n))
+  | App m (Lam n) => option_map (fun m' => App m' (Lam n)) (sos_step m)
+  | App m n => option_map (fun n' => App m n') (sos_step n) 
+  end.
+
+Fixpoint closed (x:nat) (m:tm) : bool :=
+  match m with
+  | Var y => leb (S y) x
+  | Lam m => closed (S x) m
+  | App m n => andb (closed x m) (closed x n)
+  end.
+
+Definition TM : State :=
+  {| st_ty := tm
+   ; st_dec := tm_eq_dec
+   ; st_wf m := closed 0 m = true
+  |}.
+
+Require Omega.
+
+Lemma closed_weaken : forall m x,
+  closed x m = true ->
+  closed (S x) m = true.
+Proof.
+  induction m.
+  - unfold closed. intros. apply leb_iff. apply leb_iff in H. omega.
+  - intros. apply IHm. simpl in H. assumption.
+  - intros. simpl. rewrite IHm1, IHm2; auto; simpl in *.
+    + destruct (closed x m2); auto.  destruct (closed x m1); inversion H. 
+    + destruct (closed x m1); auto.
+Qed.
+
+Lemma substitution : forall m n x,
+  closed x (Lam m) = true ->
+  closed x n = true ->
+  closed x (csubst x m n) = true.
+Proof.
+  induction m.
+  - intros.
+    unfold csubst. destruct (eq_nat_dec x n) as [Heqn|Heqn].
+    subst. assumption.
+    unfold closed. unfold closed in H. 
+    apply leb_iff. apply leb_iff in H. omega.
+  - simpl. intros. apply IHm; auto.
+    apply closed_weaken. assumption.
+  - simpl. intros. rewrite IHm1, IHm2; auto.
+    + simpl. destruct (closed (S x) m2); auto. 
+      destruct (closed (S x) m1); inversion H.
+    + simpl. destruct (closed (S x) m1); auto. 
+Qed.    
+
+Definition SOS : Mach TM.
+Proof.
+  refine (Build_Mach TM sos_step _).
+  induction x; simpl; auto.
+  intros Hwf.
+  destruct x1.
+  - inversion Hwf.
+  - destruct x2.
+    + simpl in Hwf. destruct (closed 1 x1); inversion Hwf.
+    + apply Bool.andb_true_iff in Hwf.
+      apply substitution; tauto.
+    + destruct (sos_step (App _ _)) eqn:Heq' in *.
+      apply Bool.andb_true_iff in Hwf.
+      simpl. apply Bool.andb_true_iff. split.
+      simpl in Hwf; tauto.
+      apply IHx2; tauto.
+      simpl; auto.
+  - destruct x2.
+    + simpl; auto.
+    + destruct (sos_step (App _ _)) eqn:Heq' in *.
+      apply Bool.andb_true_iff in Hwf.
+      simpl. apply Bool.andb_true_iff. tauto.
+      simpl. auto.
+    + destruct (sos_step (App x2_1 _)) eqn:Heq' in *.
+      apply Bool.andb_true_iff in Hwf.
+      simpl. apply Bool.andb_true_iff. tauto.
+      simpl. auto.
+Defined.
+
+
+Inductive clo := Clo : tm -> list clo -> clo.
+
+Inductive frame :=
+| farg : clo -> frame
+| ffun : clo -> frame.
+
+Definition cek := (clo * list frame)%type.
+
+Fixpoint cek_step (m:tm) (e:list clo) (k:list frame) : option cek :=
+  match m, k with
+  | Var x, _ => option_map (fun c => (c, k)) (nth_error e x)
+  | Lam f, farg (Clo m' e')::k' => 
+    Some (Clo m' e', ffun (Clo (Lam f) e)::k')
+  | Lam m', ffun (Clo (Lam f) e')::k' =>
+    Some (Clo f (Clo (Lam m') e::e'), k')
+  | App m' v, _ =>
+    Some (Clo m' e, (farg (Clo v e))::k)
+  | _, _ => None
+  end.
+
+End EXAMPLES.
